coq/cclc/cclc_soundness.v
@@ -3,7 +3,9 @@ From Coq Require Import ssrfun Utf8 Classical.
 Require Import AutosubstSsr ARS 
   clc_context clc_ast clc_confluence clc_subtype clc_typing
   clc_weakening clc_substitution clc_inversion clc_validity
-  cclc_ast cclc_dual cclc_typing.
+  clc_soundness clc_eval
+  clc_linearity cclc_ast cclc_dual cclc_typing cclc_weakening 
+  cclc_substitution cclc_linearity.
 
 Set Implicit Arguments.
 Unset Strict Implicit.
@@ -14,13 +16,12 @@ Proof.
   elim; move=>*; eauto using congr0.
 Qed.
 
-Lemma cong0_type Γ p q : 
-  ok Γ -> Γ ⊢ p -> congr0 p q -> Γ ⊢ q.
+Lemma congr0_type Γ p q : 
+  Γ ⊢ p -> congr0 p q -> Γ ⊢ q.
 Proof with eauto using cclc_type, congr0.
-  move=>wf ty. elim: ty wf q=>{Γ p}.
-  move=>Γ m A s tym wf q cr. inv cr.
-  move=>Γ1 Γ2 Γ p q mrg typ ihp tyq ihq wf q0 cr. 
-  have[wf1 wf2]:=merge_context_ok_inv mrg wf. inv cr.
+  move=>ty. elim: ty q=>{Γ p}.
+  move=>Γ m A s tym q cr. inv cr.
+  move=>Γ1 Γ2 Γ p q mrg typ ihp tyq ihq q0 cr. inv cr.
   { econstructor.
     apply: merge_sym...
     all: eauto. }
@@ -40,13 +41,122 @@ Proof with eauto using cclc_type, congr0.
     exact: mrg1.
     all: eauto. }
   { inv typ.
-    econstructor.
-    exact: H0.
+    have[_[e1 e2]]:=merge_re_re mrg.
     have mrg': 
       Ch A.[ren (+1)] :L Ch B :L Γ1 ∘ _: _: Γ2 => 
       Ch A.[ren (+1)] :L Ch B :L Γ.
       repeat econstructor; eauto.
+    econstructor.
+    exact: H0.
+    rewrite<-e1; eauto.
+    rewrite<-e1; eauto.
     econstructor...
-    apply strengthen.
+    replace q.[ren (+2)]%P 
+      with q.[ren (+1)].[ren (+1)]%P.
+    apply: weakeningN.
+    apply: weakeningN...
+    rewrite proc_subst_comp.
+    by asimpl. }
+  { econstructor... }
+  { econstructor.
+    apply: mrg.
+    apply: ihp...
+    apply: congr0_sym...
+    apply: ihq...
+    apply: congr0_sym... }
+  move=>Γ p A B i d tyA tyB typ ihp q cr. inv cr.
+  { inv typ. 
+    inv H1; inv H5.
+    { have[_[e1 e2]]:=merge_re_re H2.
+      econstructor.
+      apply: H2.
+      econstructor...
+      rewrite e1...
+      rewrite e1...
+      apply: strengthen.
+      apply: strengthen.
+      rewrite proc_subst_comp.
+      by asimpl. }
+    { have os:of_sort (_: Ch B :L Γ2) 1 (Some L).
+        repeat econstructor.
+      have:=linearity H4 os. 
+      have->//:=iren_occurs q0 iren1. }
+    { have os:of_sort (Ch A.[ren (+1)] :L _: Γ2) 0 (Some L).
+        econstructor.
+      have:=linearity H4 os.
+      have->//:=iren_occurs q0 iren0. }
+    { have os:of_sort (Ch A.[ren (+1)] :L Ch B :L Γ2) 0 (Some L).
+        econstructor.
+      have:=linearity H4 os.
+      have->//:=iren_occurs q0 iren0. } }
+  { econstructor; eauto. }
+  { econstructor; eauto.
+    apply: ihp; eauto.
+    apply: congr0_sym... }
+Qed.
+
+Lemma congr_type Γ p q : 
+  Γ ⊢ p -> p ≡ q -> Γ ⊢ q.
+Proof.
+  move=>ty e. elim: e Γ ty=>//={q}.
+  move=>y z e ih cr Γ typ.
+    apply: congr0_type.
+    apply: ih; eauto.
+    eauto.
+  move=>y z e ih cr Γ typ.
+    apply: congr0_type.
+    apply: ih; eauto.
+    apply: congr0_sym; eauto.
+Qed.
+
+Lemma congr_expr_inj m p : ⟨ m ⟩ ≡ p -> p = ⟨ m ⟩.
+Proof.
+  elim=>//={p}.
+  move=>y z e1 e2 cr; subst. inv cr.
+  move=>y z e1 e2 cr; subst. inv cr.
+Qed.
+
+Lemma step_expr_inj m p : 
+  ⟨ m ⟩ --> p -> exists n, p = ⟨ n ⟩ /\ m ~> n.
+Proof.
+  move e:(⟨ m ⟩)=>n st. elim: st m e=>//={n p}.
+  move=>m n st m0 [e]; subst.
+    exists n; eauto.
+  move=>p p' q q' e1 st ih e2 m e3; subst.
+  move/congr_expr_inj in e1; subst.
+  have[n[e st']]:=ih _ erefl; subst.
+  move/congr_expr_inj in e2; subst.
+  by exists n.
+Qed.
+
+Theorem subject_step Γ p q :
+  ok Γ -> Γ ⊢ p -> p --> q -> Γ ⊢ q.
+Proof.
+  move=>wf ty st. elim: st Γ ty wf=>{p q}.
+  move=>c d v val Γ ty wf. 
+  { inv ty. inv H4.
+    econstructor; eauto.
+    econstructor.
 
   }
+  move=>c d v val Γ ty wf. admit.
+  move=>c d Γ ty wf. admit.
+  move=>c d Γ ty wf. admit.
+  move=>m n st Γ ty wf. inv ty.
+    econstructor.
+    apply: subject_step; eauto.
+  move=>o p q st ih Γ ty wf. inv ty.
+    have[wf1 wf2]:=merge_context_ok_inv H1 wf.
+    econstructor; eauto.
+  move=>p q st ih Γ ty wf. inv ty.
+    econstructor; eauto.
+    have tyA:=clc_weakening.weakeningN H1.
+    apply: ih; eauto.
+    econstructor.
+    econstructor; eauto.
+    asimpl in tyA; eauto.
+  move=>p p' q q' e1 st ih e2 Γ typ wf.
+    have typ':=congr_type typ e1.
+    have tyq':=ih _ typ' wf.
+    have//:=congr_type tyq' e2.
+Qed.
